Kill one admit, remove lemma proofs from fsti

src/lib/kuiper/Kuiper.Approximates.fst
@@ -61,3 +61,16 @@ instance real_like_u8 : real_like u8 = {
 let real_like_u16 : real_like u16 = magic()
 let real_like_u32 : real_like u32 = magic()
 let real_like_u64 : real_like u64 = magic()
+
+let real_seq_sum_append
+  (r1 r2 : seq Real.real)
+  : Lemma (ensures real_seq_sum (r1 `Seq.append` r2) == real_seq_sum r1 +. real_seq_sum r2)
+          (decreases Seq.length r1)
+  = lemma_seq_fold_left_sum 0.0R (+.) r1 r2
+
+let seq_approximates_append (#a:Type) {| scalar a, real_like a |}
+  (s1 s2 : a) (r1 r2 : seq Real.real)
+  : Lemma (requires s1 `approximates` real_seq_sum r1 /\ s2 `approximates` real_seq_sum r2)
+          (ensures (s1 `add` s2) `approximates` real_seq_sum (r1 `Seq.append` r2))
+  = a_add s1 s2 (real_seq_sum r1) (real_seq_sum r2);
+    real_seq_sum_append r1 r2
